revising llist, using an option instead of null

pulse/share/steel/examples/pulse/lib/Pulse.Lib.LinkedList.fst
@@ -1,73 +1,79 @@
 module Pulse.Lib.LinkedList
 open Pulse.Lib.Pervasives
+module T = FStar.Tactics
 
 noeq
-type ll (t:Type0) = {
+type node (t:Type0) = {
     head : t;
     tail : llist t;
 }
 
-and llist (t:Type0) = ref (option (ll t))
+and node_ptr (t:Type0) = ref (node t)
 
-let mk_ll #t (hd:t) (tl:llist t) : Tot (ll t)
+//A nullable pointer to a node
+and llist (t:Type0) = option (node_ptr t)
+
+let mk_node #t (hd:t) (tl:llist t) : Tot (node t)
   = {head=hd; tail=tl}
 
 let rec is_list #t (x:llist t) (l:list t)
   : Tot vprop (decreases l)
   = match l with
-    | [] -> pts_to x None
+    | [] -> pure (x == None)
     | head::tl -> 
-     exists_ (fun (tail:llist t) -> 
-        pts_to x (Some (mk_ll head tail)) **
+      exists_ (fun (v:node_ptr t) ->
+      exists_ (fun (tail:llist t) ->
+        pure (x == Some v) **
+        pts_to v (mk_node head tail) **
         is_list tail tl
-    )
-
-let is_list_cases_opt #t (x:llist t) (l:list t) (v:option (ll t)) =
-    match v with
-    | None -> pure (l == [])
-    | Some v -> 
-        exists_ (fun (tl:list t) ->
-            pure (l == v.head::tl) **
-            is_list v.tail tl
-             )
+    ))
 
 
 let is_list_cases #t (x:llist t) (l:list t)
   : Tot vprop 
-  = exists_ (fun (v:option (ll t)) ->
-     pts_to x v **
-     is_list_cases_opt x l v)
+  = match x with
+    | None -> pure (l == [])
+    | Some v -> 
+      exists_ (fun (n:node t) ->
+      exists_ (fun (tl:list t) ->
+        pts_to v n **
+        pure (l == n.head::tl) **
+        is_list n.tail tl
+      ))
 
-//open FStar.Tactics
-module T = FStar.Tactics
 
 
 let unfold_is_list_cons #t (x:llist t) (head:t) (tl:list t)
-  : Lemma (is_list x (head::tl) ==
-            (exists_ (fun (tail:llist t) -> 
-                pts_to x #full_perm (Some (mk_ll head tail)) **
-                is_list tail tl
-            )))
+  :  Lemma (is_list x (head::tl) ==
+            exists_ (fun (v:node_ptr t) ->
+                exists_ (fun (tail:llist t) ->
+                    pure (x == Some v) **
+                    pts_to v (mk_node head tail) **
+                    is_list tail tl
+                )))
   = assert (is_list x (head::tl) ==
-            (exists_ (fun (tail:llist t) -> 
-                pts_to x #full_perm (Some (mk_ll head tail)) **
-                is_list tail tl)))
-    by (T.trefl())
+            exists_ (fun (v:node_ptr t) ->
+                exists_ (fun (tail:llist t) ->
+                    pure (x == Some v) **
+                    pts_to v (mk_node head tail) **
+                    is_list tail tl
+                )))
+    by (T.norm [delta_only [`%is_list]; zeta;iota]; T.dump "A") //trefl())
 
 ```pulse
 ghost
 fn elim_is_list_nil (#t:Type0) (x:llist t) 
   requires is_list x []
-  ensures pts_to x None
+  ensures pure(x == None)
 {
-   unfold (is_list x [])
+   rewrite (is_list x []) as pure (x == None)
 }
 ```
 
 ```pulse
 ghost
-fn intro_is_list_nil (#t:Type0) (x:llist t)
-    requires pts_to x None
+fn intro_is_list_nil (#t:Type0) (x:(x:llist t { x == None }))
+    requires emp
     ensures is_list x []
 {
     fold (is_list x [])
@@ -76,32 +82,40 @@ fn intro_is_list_nil (#t:Type0) (x:llist t)
 
 ```pulse
 ghost
-fn elim_is_list_cons (#t:Type0) (x:llist t) (hd:t) (tl:list t)
-  requires is_list x (hd::tl)
-  ensures exists (tail:llist t). pts_to x (Some (mk_ll hd tail)) ** is_list tail tl
+fn elim_is_list_cons (#t:Type0) (x:llist t) (head:t) (tl:list t)
+  requires is_list x (head::tl)
+  ensures exists (v:node_ptr t) (tail:llist t).
+            pure (x == Some v) **
+            pts_to v (mk_node head tail) **
+            is_list tail tl
 {
 //   rewrite (is_list x (hd::tl))
 //     as exists (tail:llist t). pts_to x (Some (mk_ll hd tail)) ** is_list tail tl
 //     (by T.norm ())
+    //unfold (is_list #t x (head::tl));
     admit()
 }
 ```
 
 ```pulse
 ghost
-fn intro_is_list_cons (#t:Type0) (x:llist t) (tail:llist t) (#hd:t) (#tl:list t)
-    requires pts_to x (Some (mk_ll hd tail)) ** is_list tail tl
-    ensures is_list x (hd::tl)
+fn intro_is_list_cons (#t:Type0) (v:node_ptr t) (#tail:llist t) (#hd:t) (#tl:list t)
+    requires pts_to v (mk_node hd tail) ** is_list tail tl
+    ensures is_list (Some v) (hd::tl)
 {
-    // rewrite (exists (tail:llist t). 
-    //             pts_to x (Some (mk_ll hd tail)) **
-    //             is_list tail tl)
-    //   as is_list x (hd::tl);
+//     assert (exists (v:node_ptr t) (tail:llist t).
+//         pure (Some v == Some v) **
+//         pts_to v (mk_node hd tail) **
+//         is_list tail tl);
     admit()
+//    fold // [iota] 
+//      (is_list (Some v) (hd::tl))
 }
 ```
+let elim_false (p:vprop) : stt_ghost unit emp_inames (pure False) (fun _ -> p) = Pulse.Lib.Core.elim_false unit (fun _ -> p)
+let drop (p:vprop) : stt_ghost unit emp_inames p (fun _ -> emp) = admit()
 
-
+// #push-options "--ext 'pulse:env_on_err'"
 ```pulse
 ghost
 fn cases_of_is_list (#t:Type) (x:llist t) (l:list t)
@@ -109,85 +123,95 @@ fn cases_of_is_list (#t:Type) (x:llist t) (l:list t)
     ensures is_list_cases x l
 {
     match l {
-    Nil -> { 
-      rewrite (is_list x l) as (is_list x []);
-      elim_is_list_nil x;
-      fold (is_list_cases_opt x l None);
-      fold (is_list_cases x l);
-    }
-    Cons head tl -> { 
-      rewrite (is_list x l) as (is_list x (head::tl));
-      elim_is_list_cons x head tl;
-      with tail. assert is_list tail tl;   
-      let v = mk_ll head tail;
-      rewrite (is_list tail tl) as (is_list v.tail tl);
-      fold (is_list_cases_opt x l (Some v));
-      fold (is_list_cases x l);
-    }
+        Nil -> { 
+            rewrite (is_list x l) as (is_list x []);
+            elim_is_list_nil x;
+            rewrite (pure (l == [])) as (is_list_cases x l);
+        }
+        Cons head tl -> { 
+            rewrite (is_list x l) as (is_list x (head::tl));
+            elim_is_list_cons x head tl;
+            assert pure (Some? x);
+            match x {
+                None -> {  
+                    elim_false (is_list_cases x l);
+                    with tail. assert(is_list tail tl);
+                    drop (is_list tail tl);
+                    with v. assert (pts_to v (mk_node head tail));
+                    drop (pts_to v (mk_node head tail));
+                }
+                Some v -> { 
+                    with tail. assert (is_list #t tail tl);
+                    with w. assert (pts_to w (mk_node head tail));
+                    rewrite (pts_to w (mk_node head tail)) as
+                            (pts_to v (mk_node head tail));
+                    rewrite (is_list tail tl) as 
+                            (is_list (mk_node head tail).tail tl);
+                    fold (is_list_cases (Some v) l);
+                    rewrite (is_list_cases (Some v) l) as
+                            (is_list_cases x l)
+                }
+            }
+        }
     }
 }
 ```
 
 ```pulse
 ghost
-fn is_list_of_cases (#t:Type) (x:llist t) (l:list t) (v:option (ll t))
-    requires pts_to x v ** is_list_cases_opt x l v
+fn is_list_of_cases (#t:Type) (x:llist t) (l:list t)
+    requires is_list_cases x l
     ensures is_list x l
 {
-    match v {
-    None -> { 
-      rewrite (is_list_cases_opt x l v) as (pure (l==[]));
-      rewrite (pts_to x v) as (is_list x l);
-    }
-    Some vl -> {
-      rewrite (is_list_cases_opt x l v) as
-              (is_list_cases_opt x l (Some vl));
-      unfold  (is_list_cases_opt x l (Some vl));
-      with tl. assert is_list vl.tail tl;
-      assert pure (l == vl.head::tl);
-      rewrite (pts_to x v) as (pts_to x (Some (mk_ll vl.head vl.tail)));
-      intro_is_list_cons x vl.tail;
-    }
+    match x {
+        None -> { 
+            rewrite (is_list_cases x l) as pure (l==[]);
+            rewrite (pure (x == None)) as (is_list x []);
+        }
+        Some vl -> {
+            rewrite (is_list_cases x l) as (is_list_cases (Some vl) l);
+            unfold (is_list_cases (Some vl) l);
+            with n. assert (pts_to vl n);
+            with tl. assert (is_list n.tail tl);
+            rewrite (pts_to vl n) as (pts_to vl (mk_node n.head n.tail));
+            intro_is_list_cons vl;
+            rewrite (is_list (Some vl) (n.head::tl)) as (is_list x l);
+        }
     }
 }
 ```
 
+
 ```pulse
-fn read_head (#t:Type) (x:llist t) (#l:erased (list t))
-    requires is_list x l
-    returns v:option (ll t)
-    ensures pts_to x v ** is_list_cases_opt x l v
+ghost
+fn is_list_cases_none (#t:Type) (x:llist t) (#l:list t)
+    requires is_list x l ** pure (x == None)
+    ensures is_list x l ** pure (l == [])
 {
     cases_of_is_list x l;
-    unfold (is_list_cases x l);
-    let v = !x;
-    v
+    rewrite (is_list_cases x l) as pure (l == []);
+    intro_is_list_nil x;
 }
 ```
 
-```pulse
-ghost
-fn is_list_cases_none (#t:Type) (x:llist t) (#l:list t) (#v:option (ll t))
-    requires is_list_cases_opt x l v ** pure (v == None)
-    ensures pure (l == [])
-{
-    rewrite (is_list_cases_opt x l v) as
-            (is_list_cases_opt x l None);
-    unfold (is_list_cases_opt x l None)
-}
-```
 
 ```pulse
 ghost
-fn is_list_cases_some (#t:Type) (x:llist t) (v:ll t) (#l:list t)
-    requires is_list_cases_opt x l (Some v)
-    ensures  exists (tl:list t).
-                pure (l == v.head::tl) **
-                is_list v.tail tl
+fn is_list_cases_some (#t:Type) (x:llist t) (v:node_ptr t) (#l:list t) 
+    requires is_list x l ** pure (x == Some v)
+    ensures exists (hd:t) (tail:llist t) (tl:list t).
+                pts_to v (mk_node hd tail) **
+                pure (l == hd::tl) **
+                is_list tail tl
 {
-    unfold (is_list_cases_opt x l (Some v));
+    cases_of_is_list x l;
+    rewrite (is_list_cases x l) as (is_list_cases (Some v) l);
+    unfold (is_list_cases (Some v) l);
+    with n. rewrite (pts_to v n) as (pts_to v (mk_node #t n.head n.tail));
 }
 ```
+
+///////////////////////////////////////////////////////////////////////////////
 
 ```pulse
 fn is_empty (#t:Type) (x:llist t) 
@@ -195,16 +219,15 @@ fn is_empty (#t:Type) (x:llist t)
     returns b:bool
     ensures is_list x 'l ** pure (b <==> ('l == []))
 {
-    let v = read_head x;
-    match v {
+    match x {
         None -> {
             is_list_cases_none x;
-            intro_is_list_nil x;
             true
         }
         Some vl -> {
             is_list_cases_some x vl;
-            intro_is_list_cons x vl.tail #vl.head;
+            intro_is_list_cons vl;
+            rewrite (is_list (Some vl) 'l) as (is_list x 'l);
             false
         }
     }
@@ -228,23 +251,30 @@ fn length (#t:Type) (x:llist t)
     returns n:nat
     ensures is_list x l ** pure (n == List.Tot.length l)
 {
-   let v = read_head x;
-   match v {
+   match x {
     None -> {
         is_list_cases_none x;
-        intro_is_list_nil x;
         0
     }
     Some vl -> {
         is_list_cases_some x vl;
-        with tl. assert is_list vl.tail tl;
-        let n = perform (length_rec vl.tail tl);
-        intro_is_list_cons x vl.tail #vl.head;
+        let node = !vl;
+        with tail tl. assert (is_list #t tail tl);
+        rewrite (is_list tail tl) as (is_list #t node.tail tl);
+        let n = perform (length_rec node.tail tl);
+        rewrite (pts_to vl node) as (pts_to vl (mk_node node.head node.tail));
+        intro_is_list_cons vl;
+        rewrite (is_list (Some vl) l) as (is_list x l);
         (1 + n)
     }
    }
 }
 ```
+
+let return (#t:Type) (x:t) : stt t emp (fun y -> pure (x == y)) = admit()
+let null_llist #t : llist t = None #(node_ptr t)
+
+assume val dbg : vprop
 
 ```pulse
 fn create (t:Type)
@@ -252,9 +282,8 @@ fn create (t:Type)
     returns x:llist t
     ensures is_list x []
 {
-    let x = alloc #(option (ll t)) None;
-    intro_is_list_nil x;
-    x
+    intro_is_list_nil #t null_llist;
+    null_llist #t
 }
 ```
 
@@ -264,9 +293,9 @@ fn cons (#t:Type) (v:t) (x:llist t)
     returns y:llist t
     ensures is_list y (v::'l)
 {
-    let y = alloc #(option (ll t)) (Some (mk_ll v x));
-    intro_is_list_cons y x;
-    y
+    let y = alloc (mk_node v x);
+    intro_is_list_cons y;
+    Some y
 }
 ```
 
@@ -280,55 +309,54 @@ fn append (#t:Type) (x y:llist t)
              stt unit
                  (is_list x m ** is_list y n)
                  (fun _ -> is_list x (List.Tot.append m n))))
-    requires is_list x 'l1 ** is_list y 'l2 
+    requires is_list x 'l1 ** is_list y 'l2 ** pure (x =!= None)
     ensures is_list x (List.Tot.append 'l1 'l2)
 {
-   let vx = read_head x;
-   match vx {
-    None -> {
-        is_list_cases_none x; 
-        let vy = read_head y;
-        free y;
-        match vy {
+   match x {
+    None -> { //impossible
+        drop (is_list y 'l2)
+    }
+    Some np -> {
+        is_list_cases_some x np;
+        let node = !np;
+        with tail tl. assert (is_list #t tail tl);
+        rewrite (pts_to np node) as (pts_to np (mk_node node.head node.tail));
+        rewrite (is_list tail tl) as (is_list #t node.tail tl);
+        match node.tail {
             None -> {
-                is_list_cases_none y;
-                intro_is_list_nil x;
+                is_list_cases_none node.tail;
+                drop (is_list node.tail tl);
+                np := mk_node node.head y;
+                intro_is_list_cons np #y;
+                with l. rewrite (is_list (Some np) l) as (is_list x l);
             }
-            Some vly -> {
-                is_list_cases_some y vly;
-                x := Some vly;
-                rewrite (pts_to x (Some vly))
-                    as  (pts_to x (Some (mk_ll vly.head vly.tail)));
-                intro_is_list_cons x vly.tail;
+            Some _ -> {
+                perform (append_rec node.tail y tl 'l2);
+                intro_is_list_cons np;
+                with l. rewrite (is_list (Some np) l) as (is_list x l);
             }
         }
-    }
-    Some vl -> {
-        is_list_cases_some x vl;
-        with tl. assert is_list vl.tail tl;
-        perform (append_rec vl.tail y tl 'l2);
-        intro_is_list_cons x vl.tail #vl.head;
     }
    }
 }
 ```
 
-let rec take (n:nat) (l:list 't { n < List.Tot.length l })
-  : list 't
-  = if n = 0 then []
-    else List.Tot.hd l :: take (n-1) (List.Tot.tl l)
+// let rec take (n:nat) (l:list 't { n < List.Tot.length l })
+//   : list 'tg
+//   = if n = 0 then []
+//     else List.Tot.hd l :: take (n-1) (List.Tot.tl l)
 
- let rec drop (n:nat) (l:list 't { n < List.Tot.length l })
-  : list 't
-  = if n = 0 then l
-    else drop (n-1) (List.Tot.tl l)
+//  let rec drop (n:nat) (l:list 't { n < List.Tot.length l })
+//   : list 't
+//   = if n = 0 then l
+//     else drop (n-1) (List.Tot.tl l)
        
-```pulse
-fn split (#t:Type) (x:llist t) (n:nat) (#l:(l:erased (list t) { n < List.Tot.length l }))
-    requires is_list x l
-    returns y:llist t
-    ensures is_list x (take n l) ** is_list y (drop n l)
-{
-    admit()
-}
-```
+// ```pulse
+// fn split (#t:Type) (x:llist t) (n:nat) (#l:(l:erased (list t) { n < List.Tot.length l }))
+//     requires is_list x l
+//     returns y:llist t
+//     ensures is_list x (take n l) ** is_list y (drop n l)
+// {
+//     admit()
+// }
+// ```
